yarinaoshi

src/ntac/interactive.lean
@@ -10,6 +10,7 @@ open interactive.types (texpr location using_ident with_ident_list only_flag ide
 open lean.parser
 local postfix `?`:9001 := optional
 local postfix *:9001 := many
+local prefix `#`:0 := ntac.henkan
 
 namespace ntac
 --meta def trace_state {α : Type}
@@ -22,7 +23,7 @@ namespace interactive
 := henkan tactic.interactive.induction -/
 
 meta def getgoal1 : ntac expr := 
-do g::_ ← henkan get_goals,
+do g::_ ← # get_goals,
 return g
 
 meta def getgoal1_or_done : ntac goal_tree := 
@@ -33,7 +34,7 @@ return $ match gs with
 end
 -- meta def exact (e : expr) (md := semireducible) : ntac unit := 
 -- do tg ← getgoal1,
---    ret ← henkan $ tactic.exact e md,
+--    ret ← # tactic.exact e md,
 --    kata ← henkan (infer_type e),
 --    replc_ntac tg (goal_tree.exact e)
 meta def skiptgt : ntac unit :=
@@ -42,32 +43,32 @@ replc_ntac hg $ goal_tree.skip $ goal_tree.unres hg
 
 meta def exact (q : parse texpr) : ntac unit :=
 do tg ← getgoal1,
-tgt : expr ← henkan target,
-   e ← henkan $ i_to_expr_strict ``(%%q : %%tgt),
-   henkan $ tactic.exact e,
-   kata ← henkan (infer_type e),
+tgt : expr ← # target,
+   e ← # i_to_expr_strict ``(%%q : %%tgt),
+   # tactic.exact e,
+   kata ← # infer_type e,
    replc_ntac tg (goal_tree.exact e)
 
 meta def «from» := exact
 meta def admit : ntac unit :=
-henkan $  target >>= tactic.exact ∘ expr.mk_sorry
+#  target >>= tactic.exact ∘ expr.mk_sorry
 
 
 meta def «sorry» : ntac unit := admit
 
 meta def induction (hp : parse cases_arg_p) (rec_name : parse using_ident) (ids : parse with_ident_list)
   (revert : parse $ (optional (tk "generalizing" *> lean.parser.many lean.parser.ident))) : ntac unit := 
-  henkan $ tactic.interactive.induction hp rec_name ids revert
+  # tactic.interactive.induction hp rec_name ids revert
 
 meta def aa : ntac unit :=
 fail "assumption tactic failed"
 
 meta def get_goal_tree_expr_list (goals : list(name × expr)): ntac (list (goal_tree × expr)) :=
 do
-goal2 ← goals.mfilter $ λ ⟨n, m⟩, bnot <$> (henkan $ is_assigned m),
-goal2type ← henkan $ monad.sequence $ list.map (λ nex:name × expr, infer_type nex.2) goal2 ,
+goal2 ← goals.mfilter $ λ ⟨n, m⟩, bnot <$> (# is_assigned m),
+goal2type ← # monad.sequence $ list.map (λ nex:name × expr, infer_type nex.2) goal2 ,
 let goal2unres := list.map (λ nex:name × expr, goal_tree.unres $ nex.2) goal2 in
-return $  list.zip goal2unres goal2type
+return $ list.zip goal2unres goal2type
 
 -- meta def assumption2 : ntac unit :=
 -- henkan1 "assum" tactic.interactive.assumption
@@ -76,10 +77,10 @@ private meta def concat_tags (tac : ntac (list (name × expr))) : ntac unit :=
 let s := (do in_tag ← henkan get_main_tag,
       r ← tac,
       /- remove assigned metavars -/
-      r ← r.mfilter $ λ ⟨n, m⟩, bnot <$> (henkan $ is_assigned m),
+      r ← r.mfilter $ λ ⟨n, m⟩, bnot <$> (# is_assigned m),
       match r with
-      | [(_, m)] := henkan $ set_tag m in_tag /- if there is only new subgoal, we just propagate `in_tag` -/
-      | _        := r.mmap' (λ ⟨n, m⟩, henkan $ set_tag m (n::in_tag))
+      | [(_, m)] := # set_tag m in_tag /- if there is only new subgoal, we just propagate `in_tag` -/
+      | _        := r.mmap' (λ ⟨n, m⟩, # set_tag m (n::in_tag))
       end) in
 mcond (henkan tags_enabled)
   s
@@ -89,30 +90,30 @@ meta def assumption : ntac unit :=
 do { ctx ← henkan local_context,
      tg ← getgoal1,
      t   ← henkan target,
-     H   ← henkan $ find_same_type t ctx,
-     ty ← henkan $ infer_type H,
+     H   ← # find_same_type t ctx,
+     ty ← # infer_type H,
      replc_ntac tg (goal_tree.assumption t),--t janakute ty?
-     henkan $ tactic.exact H}
+     # tactic.exact H}
 <|> fail "assumption tactic failed"
 
-meta def rw (q : parse interactive.rw_rules) (l : parse location) (cfg : rewrite_cfg := {}) : ntac unit := do tg ← getgoal1, replc_ntac tg $ goal_tree.rewrite $ goal_tree.unres tg,henkan $ interactive.rw q l cfg
-meta def delta (q : parse ident*) (l : parse location) (cfg : rewrite_cfg := {}) : ntac unit := henkan $ interactive.delta q l
+meta def rw (q : parse interactive.rw_rules) (l : parse location) (cfg : rewrite_cfg := {}) : ntac unit := do tg ← getgoal1, replc_ntac tg $ goal_tree.rewrite $ goal_tree.unres tg,# interactive.rw q l cfg
+meta def delta (q : parse ident*) (l : parse location) (cfg : rewrite_cfg := {}) : ntac unit := # interactive.delta q l
 meta def simp (use_iota_eqn : parse $ (tk "!")?) (no_dflt : parse only_flag) (hs : parse simp_arg_list) (attr_names : parse with_ident_list)
               (locat : parse location) (cfg : simp_config_ext := {}) : ntac unit := 
               do tg ← getgoal1,
-              --(all_hyps, s, u) ← henkan $ mk_simp_set_core no_dflt attr_names hs tt,
-              --(hss, gex, hex, all_hyps) ← henkan $ decode_simp_arg_list_with_symm hs,
-              --gg ← henkan $ monad.sequence $ list.map (λ pe, tactic.to_expr pe tt ff) $ list.map prod.fst hss,
-              henkan $ interactive.simp use_iota_eqn no_dflt hs attr_names locat cfg,
+              --(all_hyps, s, u) ← # mk_simp_set_core no_dflt attr_names hs tt,
+              --(hss, gex, hex, all_hyps) ← # decode_simp_arg_list_with_symm hs,
+              --gg ← # monad.sequence $ list.map (λ pe, tactic.to_expr pe tt ff) $ list.map prod.fst hss,
+              # interactive.simp use_iota_eqn no_dflt hs attr_names locat cfg,
               ng ← getgoal1_or_done,
               replc_ntac tg $ goal_tree.simp ng
 meta def simpa (use_iota_eqn : parse $ (tk "!")?) (no_dflt : parse only_flag)
   (hs : parse simp_arg_list) (attr_names : parse with_ident_list)
-  (tgt : parse (tk "using" *> texpr)?) (cfg : simp_config_ext := {}) : ntac unit := henkan $ interactive.simpa use_iota_eqn no_dflt hs attr_names tgt cfg
+  (tgt : parse (tk "using" *> texpr)?) (cfg : simp_config_ext := {}) : ntac unit := # interactive.simpa use_iota_eqn no_dflt hs attr_names tgt cfg
 
 meta def rewrite (q : parse rw_rules) (l : parse location) (cfg : rewrite_cfg := {}) : ntac unit :=
  do tg ← getgoal1,
- henkan $ interactive.rewrite q l cfg,
+ # interactive.rewrite q l cfg,
     ng ← getgoal1_or_done,
     replc_ntac tg $ goal_tree.simp ng
 
@@ -121,15 +122,15 @@ rewrite q l cfg >> try assumption
 
 meta def apply_mycore (e : expr) (cfg : apply_cfg := {}) : ntac (list (name × expr)) := 
 do tg ← getgoal1,
-  goals ← henkan $ tactic.apply e,
+  goals ← # tactic.apply e,
   glist ← get_goal_tree_expr_list goals,
   replc_ntac tg $ goal_tree.apply tg glist,
   return goals
-  --henkan $ interactive.concat_tags $ henkan2 $ return goals,
+  --# interactive.concat_tags $ henkan2 $ return goals,
 
 
 meta def apply  (q : parse texpr) : ntac unit :=
-concat_tags (do h ← henkan $ i_to_expr_for_apply q, apply_mycore h)
+concat_tags (do h ← # i_to_expr_for_apply q, apply_mycore h)
 meta def tact_eapply (e : expr) : ntac (list (name × expr)) :=
 apply_mycore e {new_goals := new_goals.non_dep_only}
 meta def eapply (q : parse texpr) : ntac unit :=
@@ -137,13 +138,13 @@ concat_tags (henkan (i_to_expr_for_apply q) >>= tact_eapply)
 
 meta def by_cases : parse cases_arg_p → ntac unit
 | (n, q) := concat_tags $ do
-  p ← henkan $ tactic.to_expr_strict q,
-  henkan $ tactic.by_cases p (n.get_or_else `h),
+  p ← # tactic.to_expr_strict q,
+  # tactic.by_cases p (n.get_or_else `h),
   pos_g :: neg_g :: rest ← henkan get_goals,
   return [(`pos, pos_g), (`neg, neg_g)]
 
 meta def rsimp : ntac unit := do tg ← getgoal1, 
-henkan $ tactic.rsimp,tg2 ← getgoal1,replc_ntac tg $ goal_tree.simp $ goal_tree.unres tg2
+# tactic.rsimp,tg2 ← getgoal1,replc_ntac tg $ goal_tree.simp $ goal_tree.unres tg2
 
 
 @[inline] meta def readmy : ntac format :=
@@ -156,7 +157,7 @@ result.success (to_fmt str) s
   result.success tac s
 
 meta def pp {α} [has_to_tactic_format α] (a:α) : ntac format :=
-henkan $ has_to_tactic_format.to_tactic_format a
+# has_to_tactic_format.to_tactic_format a
 
 meta def trace {α} [has_to_tactic_format α] (a : α) : ntac unit :=
 do fmt ← pp a,
@@ -171,7 +172,7 @@ meta def trace_state2 : ntac unit := henkan tactic.interactive.trace_state
 
 meta def split : ntac unit :=
 do tg ← getgoal1,
-goals ← henkan $ tactic.split,
+goals ← # tactic.split,
 glist ← get_goal_tree_expr_list goals,
 let goal_tree_new := goal_tree.apply tg glist in 
 do replc_ntac tg goal_tree_new,
@@ -179,8 +180,8 @@ do replc_ntac tg goal_tree_new,
 
 meta def intro2_core (n : name) : ntac expr :=
 do tg ← getgoal1,
- e ← henkan $ intro_core n,
- te ← henkan $ infer_type e,
+ e ← # intro_core n,
+ te ← # infer_type e,
  ng ← getgoal1,
 replc_ntac tg $ goal_tree.intro (n, te) $ goal_tree.unres ng,
 return e
@@ -198,10 +199,10 @@ do g::gs ← henkan get_goals,
    match gs with
    | [] := tac
    | _  := do
-      henkan $ set_goals [g],
+      # set_goals [g],
       a ← tac,
-      gs' ← henkan $ get_goals,
-      henkan $ set_goals (gs' ++ gs),
+      gs' ← # get_goals,
+      # set_goals (gs' ++ gs),
       return a
    end
 
@@ -213,39 +214,39 @@ do tag ← henkan get_main_tag,
      gs ← henkan get_goals,
      when (bnot gs.empty) $ do
        new_tag ← henkan get_main_tag,
-       when new_tag.empty $ henkan $ with_enable_tags (set_main_tag tag)
+       when new_tag.empty $ # with_enable_tags (set_main_tag tag)
 
 meta def intro : parse ident_? → ntac unit
 | none     := propagate_tags (intro1 >> skip)
 | (some h) := propagate_tags (intro2 h >> skip)
-meta def rintro (p :parse rintro_parse ) : ntac unit := henkan $ interactive.rintro p
-meta def ring (red : parse (tk "!")?) (SOP : parse ring.mode) (loc : parse location) : ntac unit := henkan $ interactive.ring red SOP loc 
-meta def obtain  (p : parse obtain_parse ): ntac unit := henkan $ interactive.obtain p
-meta def use (l : parse pexpr_list_or_texpr) : ntac unit := henkan $ interactive.use l
-meta def rcases (p : parse rcases_parse ) : ntac unit := henkan $ interactive.rcases p
+meta def rintro (p :parse rintro_parse ) : ntac unit := # interactive.rintro p
+meta def ring (red : parse (tk "!")?) (SOP : parse ring.mode) (loc : parse location) : ntac unit := # interactive.ring red SOP loc 
+meta def obtain  (p : parse obtain_parse ): ntac unit := # interactive.obtain p
+meta def use (l : parse pexpr_list_or_texpr) : ntac unit := # interactive.use l
+meta def rcases (p : parse rcases_parse ) : ntac unit := # interactive.rcases p
 meta def refine (q : parse texpr) : ntac unit :=
-henkan $ tactic.refine q
+# tactic.refine q
 
 meta def assert (h : name) (t : expr) : ntac expr :=
 do tg ← getgoal1,
-e ← henkan $ tactic.assert h t,
+e ← # tactic.assert h t,
 tg1::tg2::_ ← henkan get_goals,
 replc_ntac tg $ goal_tree.willhave (goal_tree.unres tg1) (goal_tree.unres tg2), return e
 meta def assertv (h : name) (t : expr) (v : expr) : ntac expr :=
 do tg ← getgoal1,
-e ← henkan $ tactic.assertv h t v,
+e ← # tactic.assertv h t v,
 tg1 ← getgoal1,
 replc_ntac tg $ goal_tree.have_ e (goal_tree.unres tg1), return e
 meta def note (h : name) (t : option expr := none) (pr : expr) : ntac expr :=
 do tg ← getgoal1,
-e ← henkan $ tactic.note h t pr,
+e ← # tactic.note h t pr,
 tg1 ← getgoal1,
 replc_ntac tg $ goal_tree.have_ e (goal_tree.unres tg1), return e
 meta def have_aux (h : parse ident?) (q₁ : parse (tk ":" *> texpr)?) (q₂ : parse $ (tk ":=" *> texpr)?) : ntac expr :=
 let h := h.get_or_else `this in
 match q₁, q₂ with
 | some e, some p := do
-  t ← henkan $ i_to_expr e,
+  t ← # i_to_expr e,
   v ←henkan $  i_to_expr ``(%%p : %%t),
   assertv h t v
 | none, some p := do
@@ -267,7 +268,7 @@ skip
 
 meta def let_aux (h : parse ident?) (q₁ : parse (tk ":" *> texpr)?) (q₂ : parse $ (tk ":=" *> texpr)?) : ntac expr :=
 let h := h.get_or_else `this in
-henkan $ match q₁, q₂ with
+# match q₁, q₂ with
 | some e, some p := do
   t ← i_to_expr e,
   v ← i_to_expr ``(%%p : %%t),
@@ -302,15 +303,15 @@ private meta def apply_num_metavars : expr → expr → nat → tactic expr
 
 meta def existsi_org (e : expr) : ntac unit :=
 do tg ← getgoal1,
-[c]     ← henkan $ target' >>= get_constructors_for | fail "existsi tactic failed, target is not an inductive datatype with only one constructor",
-   fn      ← henkan $ mk_const c,
-   fn_type ← henkan $ infer_type fn,
-   n       ← henkan $  get_arity fn,
+[c]     ← # target' >>= get_constructors_for | fail "existsi tactic failed, target is not an inductive datatype with only one constructor",
+   fn      ← # mk_const c,
+   fn_type ← # infer_type fn,
+   n       ← #  get_arity fn,
    when (n < 2) (fail "existsi tactic failed, constructor must have at least two arguments"),
-   t       ← henkan $ apply_num_metavars fn fn_type (n - 2),
+   t       ← # apply_num_metavars fn fn_type (n - 2),
    tact_eapply (expr.app t e),
-   t_type  ← henkan $ infer_type t >>= whnf,
-   e_type  ← henkan $ infer_type e,
+   t_type  ← # infer_type t >>= whnf,
+   e_type  ← # infer_type e,
    (guard t_type.is_pi <|> fail "existsi tactic failed, failed to infer type"),
    (henkan (unify t_type.binding_domain e_type) <|> fail "existsi tactic failed, type mismatch between given term witness and expected type"),
    skip
@@ -330,7 +331,7 @@ meta def existsi : parse pexpr_list_or_texpr → ntac unit
 
 meta def by_contradiction (n : parse ident?) : ntac unit :=
 do tg ← getgoal1,
-henkan $ tactic.by_contradiction (n.get_or_else `h) $> (),
+# tactic.by_contradiction (n.get_or_else `h) $> (),
 tg2 ← getgoal1,
 replc_ntac tg $ goal_tree.contra (goal_tree.unres tg2)
 
@@ -340,7 +341,7 @@ by_contradiction n
 meta def seq' (tac1 : ntac unit) (tac2 : ntac unit) : ntac unit :=
 do g::gs ← henkan get_goals,
    goal_trees_bak ← get_goal_tree,
-   henkan $ set_goals [g],
+   # set_goals [g],
    set_goal_tree $ goal_tree.unres g,
    tac1,
    goal_trees ← get_goal_tree,
@@ -349,13 +350,13 @@ do g::gs ← henkan get_goals,
    all_goals' tac2,
    goal_trees_new ← get_goal_tree,
    gs' ← henkan get_goals,
-   henkan $ set_goals (gs' ++ gs),
+   # set_goals (gs' ++ gs),
    set_goal_tree $ replc_unres g goal_trees_new goal_trees_bak
 
 meta instance : has_andthen (ntac unit) (ntac unit) (ntac unit) :=
 ⟨seq'⟩
 
-meta def rotate_left (n: nat): ntac unit:= henkan $ tactic.rotate_left n 
+meta def rotate_left (n: nat): ntac unit:= # tactic.rotate_left n 
 end interactive
 end ntac
 
